verified/secprop/conf_ni_entry.i.dfy
@@ -1,0 +1,1841 @@
+include "sec_prop.s.dfy"
+include "../pagedb.s.dfy"
+include "../entry.s.dfy"
+include "sec_prop_util.i.dfy"
+include "../smcapi.i.dfy"
+
+
+// This one's unstable so it's at the top!
+lemma lemma_userspaceExec_atkr(
+s11: state, s1':state, s12: state, s13:state, s14: state, d1:PageDb, d14: PageDb,
+s21: state, s2':state, s22: state, s23:state, s24: state, d2:PageDb, d24: PageDb,
+dispPg: PageNr, atkr: PageNr, l1p: PageNr)
+    requires ValidState(s11) && ValidState(s12) && ValidState(s13) && ValidState(s14)
+    requires ValidState(s21) && ValidState(s22) && ValidState(s23) && ValidState(s24)
+    requires validPageDb(d1) && validPageDb(d14)
+    requires validPageDb(d2) && validPageDb(d24)
+    requires SaneConstants()
+    requires s12.conf.nondet == s22.conf.nondet;
+    requires userspaceExecutionAndException'(s11, s1', s12, s14)
+    requires userspaceExecutionAndException'(s21, s2', s22, s24)
+    requires s13 == userspaceExecutionFn(s12, OperandContents(s11, OLR)).0;
+    requires s23 == userspaceExecutionFn(s22, OperandContents(s21, OLR)).0;
+    requires atkr_entry(d1, d2, dispPg, atkr)
+    requires loweq_pdb(d1, d2, atkr)
+    requires l1pOfDispatcher(d1, dispPg) == l1pOfDispatcher(d2, dispPg) == l1p
+    requires OperandContents(s11, OLR) == OperandContents(s21, OLR)
+    requires user_regs(s11.regs) == user_regs(s21.regs)
+    requires 
+        pageTableCorresponds(s12, d1, l1p) &&
+        pageTableCorresponds(s22, d2, l1p) &&
+        dataPagesCorrespond(s12.m, d1) &&
+        dataPagesCorrespond(s22.m, d2)
+    requires d14 == updateUserPagesFromState(s14, d1, dispPg);
+    requires d24 == updateUserPagesFromState(s24, d2, dispPg);
+    ensures loweq_pdb(d14, d24, atkr)
+    ensures atkr_entry(d14, d24, dispPg, atkr)
+{
+    var pc1 := OperandContents(s11, OLR);
+    var pc2 := OperandContents(s21, OLR);
+    var pt1 := ExtractAbsPageTable(s12);
+    var pt2 := ExtractAbsPageTable(s22);
+    
+    lemma_userStatesEquiv_atkr(
+        s11, s1', s12, s14, pc1, pt1, d1,
+        s21, s2', s22, s24, pc2, pt2, d2,
+        dispPg, atkr, l1p);
+
+    var user_state1 := user_visible_state(s12, pc1, pt1.v);
+    var user_state2 := user_visible_state(s22, pc2, pt2.v);
+
+    forall( n : PageNr | pageSWrInAddrspace(d1, l1p, n))
+        ensures contentsOfPage(s14, n) ==
+            contentsOfPage(s24, n)
+    {
+        var base := page_monvaddr(n);
+        forall( a : addr | a in addrsInPage(n, base) )
+            ensures s13.m.addresses[a] == s23.m.addresses[a]
+        {
+            reveal userspaceExecutionFn();
+            assert ExtractAbsPageTable(s12) == ExtractAbsPageTable(s22) by
+            {
+                lemma_eqpdb_pt_coresp(d1, d2, s12, s22, l1p, atkr);
+            }
+            var pt := ExtractAbsPageTable(s22);
+            assert pt.Just?;
+            var pages := WritablePagesInTable(fromJust(pt));
+            
+            if( PageBase(a) in pages ){
+                assert s13.m.addresses[a] ==s23.m.addresses[a];
+            } else {
+                reveal loweq_pdb();
+                lemma_data_page_eqdb_to_addrs(d1, d2, s12, s22, n, a, atkr);
+            }
+        }
+        assert s14.m == s13.m;
+        assert s24.m == s23.m;
+    }
+
+    
+    assert valAddrPage(d14, atkr) by { reveal updateUserPagesFromState(); }
+    forall( n : PageNr | pgInAddrSpc(d14, n, atkr) &&
+        d14[n].PageDbEntryTyped? &&
+        d24[n].PageDbEntryTyped?)
+        ensures d14[n].entry == d24[n].entry
+    {
+        reveal updateUserPagesFromState();
+        reveal loweq_pdb();
+        assert pageSWrInAddrspace(d1, l1p, n) <==>
+            pageSWrInAddrspace(d2, l1p, n);
+        if(pageSWrInAddrspace(d1, l1p, n)) {
+            assert d1[n].entry == d2[n].entry;
+            assert d14[n] == d1[n].(entry := d1[n].entry.(
+                contents := contentsOfPage(s14, n)));
+            assert d24[n] == d2[n].(entry := d2[n].entry.(
+                contents := contentsOfPage(s24, n)));
+            assert d14[n].entry == d24[n].entry;
+        } else {
+            assert d14[n].entry == d1[n].entry;
+            assert d24[n].entry == d2[n].entry;
+        }
+    }
+
+    forall(n : PageNr) 
+        ensures pgInAddrSpc(d14, n, atkr) <==> pgInAddrSpc(d1, n, atkr)
+        ensures pgInAddrSpc(d24, n, atkr) <==> pgInAddrSpc(d2, n, atkr) 
+        { reveal updateUserPagesFromState(); }
+
+    reveal loweq_pdb();
+    assert loweq_pdb(d14, d24, atkr);
+}
+
+lemma lemma_enter_conf_ni(s1: state, d1: PageDb, s1':state, d1': PageDb,
+                              s2: state, d2: PageDb, s2':state, d2': PageDb,
+                              dispPage: word, arg1: word, arg2: word, arg3: word,
+                              atkr: PageNr)
+    requires ni_reqs(s1, d1, s1', d1', s2, d2, s2', d2', atkr)
+    requires smc_enter(s1, d1, s1', d1', dispPage, arg1, arg2, arg3)
+    requires smc_enter(s2, d2, s2', d2', dispPage, arg1, arg2, arg3)
+    requires conf_loweq(s1, d1, s2, d2, atkr)
+    requires loweq_pdb(d1, d2, atkr)
+    requires s1.conf.nondet == s2.conf.nondet
+    ensures loweq_pdb(d1', d2', atkr)
+    ensures same_ret(s1', s2')
+    ensures InsecureMemInvariant(s1', s2')
+{
+    reveal loweq_pdb();
+    var e1, e2 := smc_enter_err(d1, dispPage, false), smc_enter_err(d2, dispPage, false);
+
+    assert e1 == KOM_ERR_SUCCESS <==> e2 == KOM_ERR_SUCCESS;
+
+    if(e1 == KOM_ERR_SUCCESS && e2 == KOM_ERR_SUCCESS) {
+        var asp1, asp2 := d1[dispPage].addrspace, d2[dispPage].addrspace;
+        assert asp1 == asp2;
+        if(asp1 == atkr) {
+            lemma_enter_conf_atkr_enter(s1, d1, s1', d1',
+                                       s2, d2, s2', d2',
+                                       dispPage, arg1, arg2, arg3, 
+                                       atkr, false);
+        } else {
+            lemma_enter_loweq_pdb_not_atkr(s1, d1, s1', d1',
+                                           s2, d2, s2', d2',
+                                           dispPage, arg1, arg2, arg3,
+                                           asp1, atkr, false);
+        }
+    }
+    if(e1 != KOM_ERR_SUCCESS && e2 != KOM_ERR_SUCCESS) {
+        assert loweq_pdb(d1', d2', atkr);
+    }
+
+}
+
+lemma
+lemma_enter_loweq_pdb_not_atkr(s1: state, d1: PageDb, s1':state, d1': PageDb,
+                               s2: state, d2: PageDb, s2':state, d2': PageDb,
+                               dispPage: word, arg1: word, arg2: word, arg3: word,
+                               asp: PageNr,atkr: PageNr, isresume:bool)
+    requires ni_reqs(s1, d1, s1', d1', s2, d2, s2', d2', atkr)
+    requires valAddrPage(d1, asp) && valAddrPage(d2, asp)
+    requires !isresume ==> smc_enter(s1, d1, s1', d1', dispPage, arg1, arg2, arg3)
+    requires !isresume ==> smc_enter(s2, d2, s2', d2', dispPage, arg1, arg2, arg3)
+    requires isresume ==> smc_resume(s1, d1, s1', d1', dispPage)
+    requires isresume ==> smc_resume(s2, d2, s2', d2', dispPage)
+    requires validPageNr(dispPage) && d1[dispPage].PageDbEntryTyped? && 
+        d2[dispPage].PageDbEntryTyped?
+    requires d1[dispPage].addrspace == asp && d2[dispPage].addrspace == asp
+    requires asp != atkr
+    requires InsecureMemInvariant(s1, s2)
+    requires loweq_pdb(d1, d2, atkr)
+    requires smc_enter_err(d1, dispPage, isresume) == KOM_ERR_SUCCESS
+            && (smc_enter_err(d2, dispPage, isresume) == KOM_ERR_SUCCESS);
+    requires s1.conf.nondet == s2.conf.nondet
+    ensures  loweq_pdb(d1', d2', atkr)
+    ensures  InsecureMemInvariant(s1', s2')
+    ensures  same_ret(s1', s2')
+{
+    if(!isresume) {
+        var s11:state, steps1: nat :|
+            preEntryEnter(s1, s11, d1, dispPage, arg1, arg2, arg3) &&
+            validEnclaveExecution(s11, d1, s1', d1', dispPage, steps1);
+        
+        var s21:state, steps2: nat :|
+            preEntryEnter(s2, s21, d2, dispPage, arg1, arg2, arg3) &&
+            validEnclaveExecution(s21, d2, s2', d2', dispPage, steps2);
+
+        assert s11.conf.nondet == s21.conf.nondet;
+        assert user_regs(s11.regs) == user_regs(s21.regs);
+
+        assert !spsr_of_state(s11).f && !spsr_of_state(s11).i &&
+            !spsr_of_state(s21).f && !spsr_of_state(s21).i by {
+            assert psr_mask_fiq(encode_mode(User)) == 0 by {
+                assert WordAsBits(0x10) == 0x10 && WordAsBits(0x40) == 0x40
+                    by { reveal WordAsBits(); }
+                lemma_BitsAndWordConversions();
+                reveal BitAnd();
+            }
+            assert psr_mask_irq(encode_mode(User)) == 0 by {
+                assert WordAsBits(0x10) == 0x10 && WordAsBits(0x80) == 0x80
+                    by { reveal WordAsBits(); }
+                lemma_BitsAndWordConversions();
+                reveal BitAnd();
+            }
+        }
+        lemma_validEnclaveEx_conf_not_atkr(s11, d1, s1', d1', s21, d2, s2', d2',
+                                         dispPage, steps1, steps2, asp, atkr);
+    } else {
+        var s11:state, steps1: nat :|
+            preEntryResume(s1, s11, d1, dispPage) &&
+            validEnclaveExecution(s11, d1, s1', d1', dispPage, steps1);
+        
+        var s21:state, steps2: nat :|
+            preEntryResume(s2, s21, d2, dispPage) &&
+            validEnclaveExecution(s21, d2, s2', d2', dispPage, steps2);
+
+        assert s11.conf.nondet == s21.conf.nondet;
+
+        lemma_validEnclaveEx_conf_not_atkr(s11, d1, s1', d1', s21, d2, s2', d2',
+                                     dispPage, steps1, steps2, asp, atkr);
+    }
+}
+
+lemma lemma_validEnclaveEx_conf_not_atkr(s1: state, d1: PageDb, s1':state, d1': PageDb,
+                                        s2: state, d2: PageDb, s2':state, d2': PageDb,
+                                        dispPg: PageNr, steps1:nat, steps2:nat,
+                                        asp: PageNr, atkr: PageNr)
+    
+    requires ValidState(s1) && ValidState(s2) &&
+             ValidState(s1') && ValidState(s2') &&
+             validPageDb(d1) && validPageDb(d2) && 
+             validPageDb(d1') && validPageDb(d2') && SaneConstants()
+    requires do_declassify()
+    requires valAddrPage(d1, asp) && valAddrPage(d2, asp)
+    requires valAddrPage(d1, atkr) && valAddrPage(d2, atkr)
+    requires finalDispatcher(d1, dispPg) && finalDispatcher(d2, dispPg)
+    requires d1[dispPg].addrspace == asp && d2[dispPg].addrspace == asp
+    requires asp != atkr
+    requires validEnclaveExecution(s1, d1, s1', d1', dispPg, steps1)
+    requires validEnclaveExecution(s2, d2, s2', d2', dispPg, steps2);
+    requires InsecureMemInvariant(s1, s2)
+    requires loweq_pdb(d1, d2, atkr)
+    requires s1.conf.nondet == s2.conf.nondet
+    requires mode_of_state(s1) != User && mode_of_state(s2) != User
+    requires !spsr_of_state(s1).f && !spsr_of_state(s1).i
+    requires !spsr_of_state(s2).f && !spsr_of_state(s2).i
+    requires s1.conf.scr == s2.conf.scr;
+    // stuff for looping over SVCs:
+    ensures  valAddrPage(d1', asp) && valAddrPage(d2', asp)
+    ensures  valAddrPage(d1', atkr) && valAddrPage(d2', atkr)
+    ensures  finalDispatcher(d1', dispPg) && finalDispatcher(d2', dispPg)
+    ensures  d1'[dispPg].addrspace == asp && d2'[dispPg].addrspace == asp
+    // Stuff we actually care about:
+    ensures  InsecureMemInvariant(s1', s2')
+    ensures  same_ret(s1', s2')
+    ensures  loweq_pdb(d1', d2', atkr)
+    decreases steps1, steps2
+{
+    reveal validEnclaveExecution();
+
+    var retToEnclave1, s15, d15 := lemma_unpack_validEnclaveExecution(
+        s1, d1, s1', d1', dispPg, steps1);
+    var retToEnclave2, s25, d25 := lemma_unpack_validEnclaveExecution(
+        s2, d2, s2', d2', dispPg, steps2);
+
+    lemma_validEnclaveExecutionStep_validPageDb(s1, d1, s15, d15, dispPg, retToEnclave1);
+    lemma_validEnclaveExecutionStep_validPageDb(s2, d2, s25, d25, dispPg, retToEnclave2);
+    lemma_validEnclaveStep_conf_not_atkr(s1, d1, s15, d15, s2, d2, s25, d25,
+        dispPg, retToEnclave1, retToEnclave2, asp, atkr);
+
+    assert retToEnclave1 == retToEnclave2;
+
+    if(retToEnclave1) {
+        lemma_validEnclaveExecution(s15, d15, s1', d1', dispPg, steps1 - 1);
+        lemma_validEnclaveExecution(s25, d25, s2', d2', dispPg, steps2 - 1);
+        lemma_validEnclaveEx_conf_not_atkr(s15, d15, s1', d1', s25, d25, s2', d2',
+                                         dispPg, steps1 - 1, steps2 - 1, asp, 
+                                         atkr);
+    } else {
+        reveal loweq_pdb();
+    }
+}
+
+lemma lemma_validEnclaveStep_conf_not_atkr(s1: state, d1: PageDb, s1':state, d1': PageDb,
+                                          s2: state, d2: PageDb, s2':state, d2': PageDb,
+                                          dispPg: PageNr, ret1:bool, ret2:bool,
+                                          asp: PageNr, atkr: PageNr)
+    requires ValidState(s1) && ValidState(s2) &&
+             ValidState(s1') && ValidState(s2') &&
+             validPageDb(d1) && validPageDb(d2) && 
+             validPageDb(d1') && validPageDb(d2') && SaneConstants()
+    requires do_declassify()
+    requires valAddrPage(d1, asp) && valAddrPage(d2, asp)
+    requires valAddrPage(d1, atkr) && valAddrPage(d2, atkr)
+    requires finalDispatcher(d1, dispPg)
+    requires finalDispatcher(d2, dispPg)
+    requires d1[dispPg].addrspace == asp && d2[dispPg].addrspace == asp
+    requires asp != atkr
+    requires InsecureMemInvariant(s1, s2)
+    requires validEnclaveExecutionStep(s1, d1, s1', d1', dispPg, ret1);
+    requires validEnclaveExecutionStep(s2, d2, s2', d2', dispPg, ret2);
+    requires loweq_pdb(d1, d2, atkr)
+    requires s1.conf.nondet == s2.conf.nondet
+    requires mode_of_state(s1) != User && mode_of_state(s2) != User
+    requires !spsr_of_state(s1).f && !spsr_of_state(s1).i
+    requires !spsr_of_state(s2).f && !spsr_of_state(s2).i
+    requires s1.conf.scr == s2.conf.scr;
+    ensures  loweq_pdb(d1', d2', atkr)
+    ensures  ret1 == ret2
+    ensures  ret1 ==> s1'.conf.nondet == s2'.conf.nondet;
+    ensures  !ret1 ==> same_ret(s1', s2')
+    ensures  valAddrPage(d1', asp)  && valAddrPage(d2', asp)
+    ensures  valAddrPage(d1', atkr) && valAddrPage(d2', atkr)
+    ensures  finalDispatcher(d1', dispPg) && finalDispatcher(d2', dispPg)
+    ensures  d1'[dispPg].addrspace == asp && d2'[dispPg].addrspace == asp
+    ensures  InsecureMemInvariant(s1', s2')
+{
+    reveal validEnclaveExecutionStep();
+    var s14, d14 :|
+        validEnclaveExecutionStep'(s1, d1, s14, d14, s1', d1',
+            dispPg, ret1);
+
+    var s24, d24 :|
+        validEnclaveExecutionStep'(s2, d2, s24, d24, s2', d2',
+            dispPg, ret2);
+
+    lemma_validEnclaveStepPrime_conf_not_atkr(
+        s1, d1, s14, d14, s1', d1',
+        s2, d2, s24, d24, s2', d2',
+        dispPg, ret1, ret2, asp, atkr);
+}
+
+lemma {:timeLimitMultiplier 3}
+lemma_validEnclaveStepPrime_conf_not_atkr(
+s11: state, d11: PageDb, s14:state, d14:PageDb, r1:state, rd1:PageDb,
+s21: state, d21: PageDb, s24:state, d24:PageDb, r2:state, rd2:PageDb,
+dispPg:PageNr, retToEnclave1:bool, retToEnclave2:bool,
+asp: PageNr, atkr: PageNr)
+    requires ValidState(s11) && ValidState(s21) &&
+             ValidState(r1)  && ValidState(r2)  &&
+             validPageDb(d11) &&
+             validPageDb(d21) && 
+             validPageDb(d14) && 
+             validPageDb(d24) && 
+             validPageDb(rd1) && 
+             validPageDb(rd2) && 
+             SaneConstants()
+    requires do_declassify()
+    requires valAddrPage(d11, asp) && valAddrPage(d21, asp)
+    requires valAddrPage(d11, atkr) && valAddrPage(d21, atkr)
+    requires finalDispatcher(d11, dispPg)
+    requires finalDispatcher(d21, dispPg)
+    requires validEnclaveExecutionStep'(s11,d11,s14,d14,r1,rd1,dispPg,retToEnclave1)
+    requires validEnclaveExecutionStep'(s21,d21,s24,d24,r2,rd2,dispPg,retToEnclave2)
+    requires InsecureMemInvariant(s11, s21)
+    requires d11[dispPg].addrspace == asp && d21[dispPg].addrspace == asp
+    requires asp != atkr
+    requires loweq_pdb(d11, d21, atkr)
+    requires s11.conf.nondet == s21.conf.nondet
+    requires mode_of_state(s11) != User && mode_of_state(s21) != User
+    // requires spsr_same(s11, s21)
+    requires s11.conf.scr == s21.conf.scr;
+    ensures  loweq_pdb(rd1, rd2, atkr)
+    ensures  InsecureMemInvariant(r1, r2)
+    ensures  retToEnclave1 == retToEnclave2
+    ensures  retToEnclave1 ==> r1.conf.scr == r2.conf.scr
+    ensures  retToEnclave1 ==> r1.conf.nondet == r2.conf.nondet
+    ensures  !retToEnclave1 ==> same_ret(r1, r2)
+    ensures  valAddrPage(rd1, asp)  && valAddrPage(rd2, asp)
+    ensures  valAddrPage(rd1, atkr) && valAddrPage(rd2, atkr)
+    ensures finalDispatcher(rd1, dispPg) && finalDispatcher(rd2, dispPg)
+    ensures  rd1[dispPg].addrspace == asp && rd2[dispPg].addrspace == asp
+    // ensures  retToEnclave1 ==> OperandContents(r1, OLR) == OperandContents(r2, OLR)
+    // ensures  retToEnclave1 ==> user_regs(r1.regs) == user_regs(r2.regs)
+{    
+    assert l1pOfDispatcher(d11, dispPg) == l1pOfDispatcher(d21, dispPg) by
+        { reveal loweq_pdb(); }
+    var l1p := l1pOfDispatcher(d11, dispPg);
+
+    assert dataPagesCorrespond(s11.m, d11);
+    assert dataPagesCorrespond(s21.m, d21);
+    
+    assert userspaceExecutionAndException(s11, s14);
+    assert userspaceExecutionAndException(s21, s24);
+    
+    reveal userspaceExecutionAndException();
+
+    var s1', s12 :| userspaceExecutionAndException'(s11, s1', s12, s14);
+    var s2', s22 :| userspaceExecutionAndException'(s21, s2', s22, s24);
+
+    var pc1 := OperandContents(s11, OLR);
+    var pc2 := OperandContents(s21, OLR);
+    
+    assert ExtractAbsPageTable(s12).Just? by {
+        assert ExtractAbsPageTable(s11).Just?;
+        assert ExtractAbsPageTable(s11) == ExtractAbsPageTable(s1');
+        assert ExtractAbsPageTable(s12) == ExtractAbsPageTable(s1');
+    }
+    var (s13, expc1, ex1) := userspaceExecutionFn(s12, pc1);
+    var (s23, expc2, ex2) := userspaceExecutionFn(s22, pc2);
+  
+    assert InsecureMemInvariant(s12, s22) by {
+        assert InsecureMemInvariant(s11, s12);
+        assert InsecureMemInvariant(s21, s22);
+    }
+
+    var pt1 := ExtractAbsPageTable(s12);
+    var pt2 := ExtractAbsPageTable(s22);
+
+    assert pageTableCorresponds(s12, d11, l1p)
+        && pageTableCorresponds(s22, d21, l1p) by
+    { 
+        assert pageTableCorresponds(s11, d11, l1p);
+        assert pageTableCorresponds(s21, d21, l1p);
+        reveal pageTableCorresponds();
+    }
+
+    assert pt1 == pt2 by {
+        lemma_eqpdb_pt_coresp_not_atkr(d11, d21, s12, s22, l1p, asp, atkr);
+    }
+
+    assert s12.conf.nondet == s22.conf.nondet;
+
+    assert InsecureMemInvariant(s13, s23) by {
+        lemma_insecure_mem_userspace(
+            s12, pc1, s13, expc1, ex1,
+            s22, pc2, s23, expc2, ex2);
+    }
+
+    assert InsecureMemInvariant(s14, s24);
+
+    assert InsecureMemInvariant(r1, r2);
+
+    assert s13.conf.nondet == s23.conf.nondet by
+    {
+        reveal userspaceExecutionFn();
+        assert s13.conf.nondet == nondet_int(s12.conf.nondet, NONDET_GENERATOR());
+        assert s23.conf.nondet == nondet_int(s22.conf.nondet, NONDET_GENERATOR());
+    }
+    
+    assert s14.conf.nondet == s24.conf.nondet;
+
+    assert ex1 == ex2 && s14.conf.ex == s24.conf.ex by {
+        lemma_decl_ex(s1', s12, s14, s2', s22, s24);
+    }
+
+    assert loweq_pdb(d14, d24, atkr) by
+    {
+        assert validPageDbs({d11,d21,d14,d24});
+        lemma_updateUserPages_conf_not_atkr(s14, d11, d14,
+            s24, d21, d24, dispPg, asp, atkr);
+    }
+
+    assert valAddrPage(d14, atkr) && valAddrPage(d24, atkr) &&
+        d14[dispPg].addrspace == asp && d24[dispPg].addrspace == asp by
+        { reveal updateUserPagesFromState(); }
+
+    assert retToEnclave1 == retToEnclave2 &&
+        (ex1 == ExSVC ==> s14.regs[R0] == s24.regs[R0]) &&
+        (ex1 == ExSVC && (s14.regs[R0] == KOM_SVC_EXIT ||
+            s14.regs[R0] == KOM_SVC_MAP_DATA ||
+            s14.regs[R0] == KOM_SVC_UNMAP_DATA ||
+            s14.regs[R0] == KOM_SVC_INIT_L2PTABLE) ==>
+            s14.regs[R1] == s24.regs[R1]) &&
+        (ex1 == ExSVC && (s14.regs[R0] == KOM_SVC_MAP_DATA ||
+            s14.regs[R0] == KOM_SVC_UNMAP_DATA ||
+            s14.regs[R0] == KOM_SVC_INIT_L2PTABLE) ==>
+            s14.regs[R2] == s24.regs[R2]) by
+    {
+        assert s14.regs[R0] == s13.regs[R0];
+        assert s24.regs[R0] == s23.regs[R0];
+        reveal userspaceExecutionFn();
+        if(ex1 == ExSVC) {
+            lemma_decl_svc_r0(s13, s14, s23, s24);
+            if(s14.regs[R0] == KOM_SVC_EXIT ||
+               s14.regs[R0] == KOM_SVC_MAP_DATA ||
+               s14.regs[R0] == KOM_SVC_UNMAP_DATA ||
+               s14.regs[R0] == KOM_SVC_INIT_L2PTABLE){
+                lemma_decl_svc_r1(s13, s14, s23, s24);
+            }
+            if(s14.regs[R0] == KOM_SVC_MAP_DATA ||
+               s14.regs[R0] == KOM_SVC_UNMAP_DATA ||
+               s14.regs[R0] == KOM_SVC_INIT_L2PTABLE){
+                lemma_decl_svc_r2(s13, s14, s23, s24);
+            }
+        }
+    }
+   
+    lemma_validEnclaveStepPrime_conf_not_atkr_retnondet(
+        s11, d11, s14, d14, r1, rd1,
+        s21, d21, s24, d24, r2, rd2,
+        dispPg, retToEnclave1, retToEnclave2, asp, atkr);
+
+}
+
+lemma lemma_updateUserPages_conf_not_atkr(
+    s14: state, d11: PageDb, d14: PageDb,
+    s24: state, d21: PageDb, d24: PageDb,
+    dispPg: PageNr, asp: PageNr, atkr: PageNr)
+requires validStates({s14, s24}) && SaneConstants()
+requires validPageDbs({d11,d21,d14,d24})
+requires finalDispatcher(d11, dispPg)
+requires finalDispatcher(d21, dispPg)
+requires valAddrPage(d11, asp) && valAddrPage(d21, asp)
+requires valAddrPage(d11, atkr) && valAddrPage(d21, atkr)
+requires d11[dispPg].addrspace == asp && d21[dispPg].addrspace == asp
+requires asp != atkr
+requires d14 == updateUserPagesFromState(s14, d11, dispPg)
+requires d24 == updateUserPagesFromState(s24, d21, dispPg)
+requires loweq_pdb(d11, d21, atkr)
+ensures  loweq_pdb(d14, d24, atkr)
+{
+    reveal updateUserPagesFromState();
+    reveal loweq_pdb();
+}
+
+lemma
+lemma_validEnclaveStepPrime_conf_not_atkr_retnondet(
+s11: state, d11: PageDb, s14:state, d14:PageDb, r1:state, rd1:PageDb,
+s21: state, d21: PageDb, s24:state, d24:PageDb, r2:state, rd2:PageDb,
+dispPg:PageNr, retToEnclave1:bool, retToEnclave2:bool,
+asp: PageNr, atkr: PageNr
+)
+    requires ValidState(s11) && ValidState(s21) &&
+             ValidState(r1)  && ValidState(r2)  &&
+             validPageDb(d11) && validPageDb(d21) &&
+             validPageDb(rd1) && validPageDb(rd2) && SaneConstants()
+    requires valAddrPage(d11, asp) && valAddrPage(d21, asp)
+    requires valAddrPage(d11, atkr) && valAddrPage(d21, atkr)
+    requires finalDispatcher(d11, dispPg)
+    requires finalDispatcher(d21, dispPg)
+    requires d11[dispPg].addrspace == asp && d21[dispPg].addrspace == asp
+    requires asp != atkr
+    requires finalDispatcher(d14, dispPg)
+    requires finalDispatcher(d24, dispPg)
+    requires valAddrPage(d14, atkr) && valAddrPage(d24, atkr);
+    requires d14[dispPg].addrspace == asp && d24[dispPg].addrspace == asp;
+    requires validEnclaveExecutionStep'(s11,d11,s14,d14,r1,rd1,dispPg,retToEnclave1)
+    requires validEnclaveExecutionStep'(s21,d21,s24,d24,r2,rd2,dispPg,retToEnclave2)
+    requires s14.conf.nondet == s24.conf.nondet 
+    requires loweq_pdb(d14, d24, atkr)
+    requires retToEnclave1 == retToEnclave2
+    requires s14.conf.ex == s24.conf.ex;
+    requires (s14.conf.ex == ExSVC) ==>
+            s14.regs[R0] == s24.regs[R0];
+    requires (s14.conf.ex == ExSVC && (s14.regs[R0] == KOM_SVC_EXIT ||
+            s14.regs[R0] == KOM_SVC_MAP_DATA ||
+            s14.regs[R0] == KOM_SVC_UNMAP_DATA ||
+            s14.regs[R0] == KOM_SVC_INIT_L2PTABLE)) ==>
+        s14.regs[R1] == s24.regs[R1]
+    requires (s14.conf.ex == ExSVC && (s14.regs[R0] == KOM_SVC_MAP_DATA ||
+              s14.regs[R0] == KOM_SVC_UNMAP_DATA ||
+              s14.regs[R0] == KOM_SVC_INIT_L2PTABLE)) ==>
+        s14.regs[R2] == s24.regs[R2]
+    ensures  loweq_pdb(rd1, rd2, atkr)
+    ensures  !retToEnclave1 ==> same_ret(r1, r2)
+    ensures  retToEnclave1 ==> r1.conf.nondet == r2.conf.nondet
+    ensures  valAddrPage(rd1, asp)  && valAddrPage(rd2, asp)
+    ensures  valAddrPage(rd1, atkr) && valAddrPage(rd2, atkr)
+    ensures finalDispatcher(rd1, dispPg) && finalDispatcher(rd2, dispPg)
+    ensures  rd1[dispPg].addrspace == asp && rd2[dispPg].addrspace == asp
+{
+    if(retToEnclave1) {
+        
+        var (retRegs1, rd1') := svcHandled(s14, d14, dispPg);
+        var (retRegs2, rd2') := svcHandled(s24, d24, dispPg);
+
+        if(s14.conf.ex == ExSVC) { 
+            lemma_svcHandled_conf_not_atkr(s14, d14, rd1',
+                s24, d24, rd2', dispPg, asp, atkr);
+        }
+
+        reveal loweq_pdb();
+        
+        assert loweq_pdb(rd1', rd2', atkr);
+        assert loweq_pdb(rd1, rd2, atkr);
+
+        assert r1.conf.nondet == r2.conf.nondet by {
+            assert s14.conf.nondet == s24.conf.nondet; 
+        }
+    } else {
+        reveal ValidRegState();
+        lemma_exceptionHandled_conf_not_atkr(
+            s14, d14, rd1, r1.regs[R0], r1.regs[R1],
+            s24, d24, rd2, r2.regs[R0], r2.regs[R1],
+            dispPg, asp, atkr);
+    }
+}
+
+lemma lemma_svcHandled_conf_not_atkr(s1: state, d1: PageDb, d1': PageDb,
+                                    s2: state, d2: PageDb, d2': PageDb,
+                                    dispPg: PageNr, asp: PageNr, atkr: PageNr)
+    requires validPageDbs({d1, d1'}) && validDispatcherPage(d1, dispPg)
+    requires validPageDbs({d2, d2'}) && validDispatcherPage(d2, dispPg)
+    requires ValidState(s1) && mode_of_state(s1) != User
+    requires ValidState(s2) && mode_of_state(s2) != User
+    requires valAddrPage(d1, asp) && valAddrPage(d2, asp)
+    requires valAddrPage(d1, atkr) && valAddrPage(d2, atkr)
+    requires finalDispatcher(d1, dispPg)
+    requires finalDispatcher(d2, dispPg)
+    requires d1[dispPg].addrspace == asp && d2[dispPg].addrspace == asp
+    requires asp != atkr
+    requires OperandContents(s1, OReg(R0)) == OperandContents(s2, OReg(R0));
+    requires (s1.regs[R0] == KOM_SVC_EXIT ||
+              s1.regs[R0] == KOM_SVC_MAP_DATA ||
+              s1.regs[R0] == KOM_SVC_UNMAP_DATA ||
+              s1.regs[R0] == KOM_SVC_INIT_L2PTABLE) ==>
+        s1.regs[R1] == s2.regs[R1]
+    requires (s1.regs[R0] == KOM_SVC_MAP_DATA ||
+              s1.regs[R0] == KOM_SVC_UNMAP_DATA ||
+              s1.regs[R0] == KOM_SVC_INIT_L2PTABLE) ==>
+        s1.regs[R2] == s2.regs[R2]
+    requires isReturningSvc(s1) && finalDispatcher(d1, dispPg)
+    requires isReturningSvc(s2) && finalDispatcher(d2, dispPg)
+    requires d1' == svcHandled(s1, d1, dispPg).1
+    requires d2' == svcHandled(s2, d2, dispPg).1
+    requires loweq_pdb(d1, d2, atkr)
+    ensures loweq_pdb(d1', d2', atkr)
+    ensures valAddrPage(d1', asp)  && valAddrPage(d2', asp)
+    ensures valAddrPage(d1', atkr) && valAddrPage(d2', atkr)
+    ensures finalDispatcher(d1', dispPg) && finalDispatcher(d2', dispPg)
+    ensures  d1'[dispPg].addrspace == asp && d2'[dispPg].addrspace == asp
+{
+
+    reveal loweq_pdb();
+    var addrspace := d1[dispPg].addrspace;
+    var call := OperandContents(s1, OReg(R0));
+    if( call  == KOM_SVC_ATTEST ) {
+        assert d1' == d1;
+        assert d2' == d2;
+    } else if( call  == KOM_SVC_VERIFY_STEP0) {
+        assert loweq_entry(d1'[dispPg].entry, d2'[dispPg].entry);
+    } else if( call  == KOM_SVC_VERIFY_STEP1) {
+        assert loweq_entry(d1'[dispPg].entry, d2'[dispPg].entry);
+    } else if( call  == KOM_SVC_VERIFY_STEP2) {
+        assert d1' == d1;
+        assert d2' == d2;
+    } else if( call == KOM_SVC_MAP_DATA) {
+        var page, mapping := s1.regs[R1], s1.regs[R2];
+        var (retDb1, retErr1) := svcMapData(d1, addrspace, page, mapping);
+        var (retDb2, retErr2) := svcMapData(d2, addrspace, page, mapping);
+        assert retErr1 == KOM_ERR_INVALID_PAGENO <==>
+            retErr2 == KOM_ERR_INVALID_PAGENO;
+        assert retErr1 == KOM_ERR_INVALID_MAPPING <==>
+            retErr2 == KOM_ERR_INVALID_MAPPING;
+        if(retErr1 == KOM_ERR_SUCCESS) {
+            assert loweq_entry(d1'[page].entry, d2'[page].entry);
+
+            var abs_mapping := wordToMapping(mapping);
+            var l11 := d1[d1[addrspace].entry.l1ptnr].entry;
+            var l12 := d2[d2[addrspace].entry.l1ptnr].entry;
+            var l1pte1 := fromJust(l11.l1pt[abs_mapping.l1index]);
+            var l1pte2 := fromJust(l12.l1pt[abs_mapping.l1index]);
+            assert loweq_entry(d1'[l1pte1].entry, d2'[l1pte2].entry);
+        }
+    } else if( call == KOM_SVC_UNMAP_DATA) {
+    } else if( call == KOM_SVC_INIT_L2PTABLE) {
+        var e1 := svcHandled(s1, d1, dispPg).0.0;
+        var e2 := svcHandled(s2, d2, dispPg).0.0;
+        reveal validPageDb();
+        assert e1 == KOM_ERR_INVALID_MAPPING <==> e2 == KOM_ERR_INVALID_MAPPING;
+        assert e1 == KOM_ERR_INVALID_PAGENO <==> e2 == KOM_ERR_INVALID_PAGENO;
+        assert e1 == KOM_ERR_ADDRINUSE <==> e2 == KOM_ERR_ADDRINUSE;
+        var page := OperandContents(s1, OReg(R1));
+        var l1index := OperandContents(s1, OReg(R2));
+        if(e1 == KOM_ERR_SUCCESS) {
+            // var l2pt := L2PTable(SeqRepeat(NR_L2PTES, NoMapping));
+            // var d1 := updatePageEntry(d, page, l2pt);
+            var l1ptnr := d1[addrspace].entry.l1ptnr;
+            assert loweq_entry(d1'[page].entry, d2'[page].entry);
+            assert loweq_entry(d1'[l1ptnr].entry, d2'[l1ptnr].entry);
+            // var d2 := installL1PTEInPageDb(d1, l1ptnr, page, l1index);
+        }
+    } else {
+    }
+}
+
+lemma lemma_exceptionHandled_conf_not_atkr(
+    s14:state, d14:PageDb, rd1:PageDb, r01:word, r11:word,
+    s24:state, d24:PageDb, rd2:PageDb, r02:word, r12:word,
+    dispPg:PageNr, asp: PageNr, atkr: PageNr)
+    requires validStates({s14, s24})
+    requires validPageDbs({d14,d24,rd1,rd2})
+    requires validDispatcherPage(d14, dispPg)
+    requires validDispatcherPage(d24, dispPg)
+    requires mode_of_state(s14) != User
+    requires mode_of_state(s24) != User
+    requires valAddrPage(d14, asp) && valAddrPage(d24, asp)
+    requires valAddrPage(d14, atkr) && valAddrPage(d24, atkr)
+    requires finalDispatcher(d14, dispPg)
+    requires finalDispatcher(d24, dispPg)
+    requires d14[dispPg].addrspace == asp && d24[dispPg].addrspace == asp
+    requires asp != atkr
+    requires (r01, r11, rd1) == exceptionHandled(s14, d14, dispPg)
+    requires (r02, r12, rd2) == exceptionHandled(s24, d24, dispPg)
+    requires s14.conf.ex == s24.conf.ex
+    requires loweq_pdb(d14, d24, atkr)
+    requires R1 in s14.regs && R1 in s24.regs
+    requires s14.conf.ex.ExSVC? ==> 
+        s14.regs[R1] == s24.regs[R1]
+    ensures  loweq_pdb(rd1, rd2, atkr)
+    ensures  r01 == r02 && r11 == r12
+    ensures  valAddrPage(rd1, asp)  && valAddrPage(rd2, asp)
+    ensures  valAddrPage(rd1, atkr) && valAddrPage(rd2, atkr)
+    ensures  finalDispatcher(rd1, dispPg) && finalDispatcher(rd2, dispPg)
+    ensures  rd1[dispPg].addrspace == asp && rd2[dispPg].addrspace == asp
+{
+    reveal loweq_pdb();
+}
+
+//-----------------------------------------------------------------------------
+// Executions of attacker conflaves beginning from low-equiv states produce 
+// low-equiv states.
+//-----------------------------------------------------------------------------
+
+
+predicate atkr_entry(d1: PageDb, d2: PageDb, disp: word, atkr: PageNr)
+{
+    validPageNr(disp) &&
+    validPageDb(d1) && validPageDb(d2) &&
+    valAddrPage(d1, atkr) && valAddrPage(d2, atkr) &&
+    d1[disp].PageDbEntryTyped? && d1[disp].entry.Dispatcher? &&
+    d2[disp].PageDbEntryTyped? && d2[disp].entry.Dispatcher? &&
+    finalDispatcher(d1, disp) && finalDispatcher(d2, disp) &&
+    d1[disp].addrspace == d2[disp].addrspace == atkr
+}
+
+
+lemma lemma_enter_conf_atkr_enter(s1: state, d1: PageDb, s1':state, d1': PageDb,
+                                 s2: state, d2: PageDb, s2':state, d2': PageDb,
+                                 dispPg: word, arg1: word, arg2: word, arg3: word,
+                                 atkr: PageNr, isresume:bool)
+    requires ni_reqs(s1, d1, s1', d1', s2, d2, s2', d2', atkr)
+    requires !isresume ==> smc_enter(s1, d1, s1', d1', dispPg, arg1, arg2, arg3)
+    requires !isresume ==> smc_enter(s2, d2, s2', d2', dispPg, arg1, arg2, arg3)
+    requires isresume ==> smc_resume(s1, d1, s1', d1', dispPg)
+    requires isresume ==> smc_resume(s2, d2, s2', d2', dispPg)
+    requires conf_loweq(s1, d1, s2, d2, atkr)
+    requires entering_atkr(d1, d2, dispPg, atkr, isresume);
+    requires s1.conf.nondet == s2.conf.nondet
+    ensures  loweq_pdb(d1', d2', atkr)
+    ensures  same_ret(s1', s2')
+    ensures  InsecureMemInvariant(s1', s2')
+{
+
+    if(!isresume) {
+        var s11:state, steps1: nat :|
+            preEntryEnter(s1, s11, d1, dispPg, arg1, arg2, arg3) &&
+            validEnclaveExecution(s11, d1, s1', d1', dispPg, steps1);
+        
+        var s21:state, steps2: nat :|
+            preEntryEnter(s2, s21, d2, dispPg, arg1, arg2, arg3) &&
+            validEnclaveExecution(s21, d2, s2', d2', dispPg, steps2);
+
+        assert s11.conf.nondet == s21.conf.nondet;
+        assert user_regs(s11.regs) == user_regs(s21.regs); // XXX WHYYYYY??
+
+        assert OperandContents(s11, OLR) == OperandContents(s21, OLR) by 
+        {
+            assert OperandContents(s11, OLR) == d1[dispPg].entry.entrypoint;
+            assert OperandContents(s21, OLR) == d2[dispPg].entry.entrypoint;
+            reveal loweq_pdb();
+        }
+        
+        assert spsr_same(s11, s21) by {
+            assert preEntryEnter(s1, s11, d1, dispPg, arg1, arg2, arg3);
+            assert preEntryEnter(s2, s21, d2, dispPg, arg1, arg2, arg3);
+            var mode1 := mode_of_state(s11);
+            var mode2 := mode_of_state(s21);
+            assert mode1 != User && mode2 != User;
+            reveal ValidSRegState();
+            assert s11.sregs[spsr(mode1)] == encode_mode(User);
+            assert s21.sregs[spsr(mode2)] == encode_mode(User);
+        }
+
+        assert !spsr_of_state(s11).f && !spsr_of_state(s11).i &&
+            !spsr_of_state(s21).f && !spsr_of_state(s21).i by {
+            assert psr_mask_fiq(encode_mode(User)) == 0 by {
+                assert WordAsBits(0x10) == 0x10 && WordAsBits(0x40) == 0x40
+                    by { reveal WordAsBits(); }
+                lemma_BitsAndWordConversions();
+                reveal BitAnd();
+            }
+            assert psr_mask_irq(encode_mode(User)) == 0 by {
+                assert WordAsBits(0x10) == 0x10 && WordAsBits(0x80) == 0x80
+                    by { reveal WordAsBits(); }
+                lemma_BitsAndWordConversions();
+                reveal BitAnd();
+            }
+        }
+        lemma_validEnclaveEx_conf(s11, d1, s1', d1', s21, d2, s2', d2',
+                                             dispPg, steps1, steps2, atkr);
+    } else {
+        var s11:state, steps1: nat :|
+            preEntryResume(s1, s11, d1, dispPg) &&
+            validEnclaveExecution(s11, d1, s1', d1', dispPg, steps1);
+        
+        var s21:state, steps2: nat :|
+            preEntryResume(s2, s21, d2, dispPg) &&
+            validEnclaveExecution(s21, d2, s2', d2', dispPg, steps2);
+
+        assert s11.conf.nondet == s21.conf.nondet;
+
+        assert d1[dispPg].entry == d2[dispPg].entry by
+            { reveal loweq_pdb(); }
+
+        assert user_regs(s11.regs) == user_regs(s21.regs) by {
+            var disp := d1[dispPg].entry;
+            assert (forall r | r in USER_REGS() :: 
+                (s11.regs[r] == disp.ctxt.regs[r] &&
+                 s21.regs[r] == disp.ctxt.regs[r]));
+            eqregs(user_regs(s11.regs), user_regs(s21.regs));
+        }
+
+        assert OperandContents(s11, OLR) == OperandContents(s21, OLR) by 
+        {   
+            assert OperandContents(s11, OLR) == d1[dispPg].entry.ctxt.pc;
+            assert OperandContents(s21, OLR) == d2[dispPg].entry.ctxt.pc;
+            reveal loweq_pdb();
+        }
+        
+        assert spsr_same(s11, s21) by {
+            var disp := d1[dispPg].entry;
+            assert preEntryResume(s1, s11, d1, dispPg);
+            assert preEntryResume(s2, s21, d2, dispPg);
+            reveal ValidSRegState();
+            var mode1 := mode_of_state(s11);
+            var mode2 := mode_of_state(s21);
+            assert mode1 != User && mode2 != User;
+            assert s11.sregs[spsr(mode1)] == disp.ctxt.cpsr;
+            assert s21.sregs[spsr(mode2)] == disp.ctxt.cpsr;
+        }
+        lemma_validEnclaveEx_conf(s11, d1, s1', d1', s21, d2, s2', d2',
+                                             dispPg, steps1, steps2, atkr);
+    }
+}
+
+lemma lemma_validEnclaveEx_conf(s1: state, d1: PageDb, s1':state, d1': PageDb,
+                                    s2: state, d2: PageDb, s2':state, d2': PageDb,
+                                    dispPg: PageNr, steps1:nat, steps2:nat,
+                                    atkr: PageNr)
+    requires ValidState(s1) && ValidState(s2) &&
+             ValidState(s1') && ValidState(s2') &&
+             validPageDb(d1) && validPageDb(d2) && 
+             validPageDb(d1') && validPageDb(d2') && SaneConstants()
+    requires atkr_entry(d1, d2, dispPg, atkr)
+    requires validEnclaveExecution(s1, d1, s1', d1', dispPg, steps1)
+    requires validEnclaveExecution(s2, d2, s2', d2', dispPg, steps2);
+    requires loweq_pdb(d1, d2, atkr)
+    requires InsecureMemInvariant(s1, s2)
+    requires s1.conf.nondet == s2.conf.nondet
+    requires OperandContents(s1, OLR) == OperandContents(s2, OLR)
+    requires user_regs(s1.regs) == user_regs(s2.regs)
+    requires mode_of_state(s1) != User && mode_of_state(s2) != User
+    requires !spsr_of_state(s1).f && !spsr_of_state(s1).i
+    requires !spsr_of_state(s2).f && !spsr_of_state(s2).i
+    requires spsr_same(s1, s2)
+    requires s1.conf.scr == s2.conf.scr;
+    ensures  atkr_entry(d1', d2', dispPg, atkr)
+    ensures  loweq_pdb(d1', d2', atkr)
+    ensures InsecureMemInvariant(s1', s2')
+    ensures same_ret(s1', s2')
+    decreases steps1, steps2
+{
+    reveal validEnclaveExecution();
+
+    var retToEnclave1, s15, d15 := lemma_unpack_validEnclaveExecution(
+        s1, d1, s1', d1', dispPg, steps1);
+    var retToEnclave2, s25, d25 := lemma_unpack_validEnclaveExecution(
+        s2, d2, s2', d2', dispPg, steps2);
+
+    lemma_validEnclaveExecutionStep_validPageDb(s1, d1, s15, d15, dispPg, retToEnclave1);
+    lemma_validEnclaveExecutionStep_validPageDb(s2, d2, s25, d25, dispPg, retToEnclave2);
+    lemma_validEnclaveStep_conf(s1, d1, s15, d15, s2, d2, s25, d25,
+        dispPg, atkr, retToEnclave1, retToEnclave2);
+
+    assert retToEnclave1 == retToEnclave2;
+
+    if(retToEnclave1) {
+        lemma_validEnclaveExecution(s15, d15, s1', d1', dispPg, steps1 - 1);
+        lemma_validEnclaveExecution(s25, d25, s2', d2', dispPg, steps2 - 1);
+        lemma_validEnclaveEx_conf(s15, d15, s1', d1', s25, d25, s2', d2',
+                                         dispPg, steps1 - 1, steps2 - 1, atkr);
+        assert loweq_pdb(d1', d2', atkr);
+    } else {
+        assert s2' == s25;
+        assert s1' == s15;
+        assert d1' == d15;
+        assert d2' == d25;
+        assert loweq_pdb(d1', d2', atkr);
+    }
+
+}
+
+lemma lemma_validEnclaveStep_conf(s1: state, d1: PageDb, s1':state, d1': PageDb,
+                                      s2: state, d2: PageDb, s2':state, d2': PageDb,
+                                      dispPage:PageNr, atkr: PageNr, ret1:bool, ret2:bool)
+    requires ValidState(s1) && ValidState(s2) &&
+             ValidState(s1') && ValidState(s2') &&
+             validPageDb(d1) && validPageDb(d2) && 
+             validPageDb(d1') && validPageDb(d2') && SaneConstants()
+    requires atkr_entry(d1, d2, dispPage, atkr)
+    requires validEnclaveExecutionStep(s1, d1, s1', d1', dispPage, ret1);
+    requires validEnclaveExecutionStep(s2, d2, s2', d2', dispPage, ret2);
+    requires loweq_pdb(d1, d2, atkr)
+    requires InsecureMemInvariant(s1, s2)
+    requires s1.conf.nondet == s2.conf.nondet
+    requires OperandContents(s1, OLR) == OperandContents(s2, OLR)
+    requires user_regs(s1.regs) == user_regs(s2.regs)
+    requires mode_of_state(s1) != User && mode_of_state(s2) != User
+    requires spsr_same(s1, s2)
+    requires s1.conf.scr == s2.conf.scr;
+    ensures  InsecureMemInvariant(s1', s2')
+    ensures  atkr_entry(d1', d2', dispPage, atkr)
+    ensures  loweq_pdb(d1', d2', atkr)
+    ensures  ret1 == ret2
+    ensures  ret1 ==> s1'.conf.scr == s2'.conf.scr;
+    ensures  ret1 ==> s1'.conf.nondet == s2'.conf.nondet
+    ensures  ret1 ==> OperandContents(s1', OLR) == OperandContents(s2', OLR)
+    ensures  ret1 ==> user_regs(s1'.regs) == user_regs(s2'.regs)
+    ensures  !ret1 ==> same_ret(s1', s2')
+{
+    reveal validEnclaveExecutionStep();
+    var s14, d14 :|
+        validEnclaveExecutionStep'(s1, d1, s14, d14, s1', d1',
+            dispPage, ret1);
+
+    var s24, d24 :|
+        validEnclaveExecutionStep'(s2, d2, s24, d24, s2', d2',
+            dispPage, ret2);
+    
+    lemma_updateUserPagesFromState_validPageDb(s14, d1, dispPage);
+    lemma_updateUserPagesFromState_validPageDb(s24, d2, dispPage);
+
+    assert validPageDb(d1);
+    assert validPageDb(d2);
+    assert validPageDb(d14);
+    assert validPageDb(d24);
+    assert validPageDb(d1');
+    assert validPageDb(d2');
+    lemma_validEnclaveStepPrime_conf(
+        s1, d1, s14, d14, s1', d1',
+        s2, d2, s24, d24, s2', d2',
+        dispPage, ret1, ret2, atkr);
+}
+
+lemma lemma_user_regs_domain(regs:map<ARMReg, word>, hr:map<ARMReg, word>)
+    requires ValidRegState(regs)
+    requires hr == user_regs(regs)
+    ensures  forall r :: r in hr <==> r in USER_REGS()
+{
+}
+
+lemma eqregs(x: map<ARMReg,word>, y: map<ARMReg,word>)
+	requires forall r :: r in x <==> r in y
+	requires forall r | r in x :: x[r] == y[r]
+	ensures x == y
+	{}
+
+lemma only_user_in_user_regs(r:ARMReg, m:mode)
+    requires r == LR(m) && m != User
+    ensures r !in USER_REGS() {}
+
+lemma lemma_exceptionTakenRegs(s3:state, ex:exception, expc:word, s4:state)
+    requires ValidState(s3) && ValidPsrWord(psr_of_exception(s3, ex))
+    requires ValidState(s4)
+    requires evalExceptionTaken(s3, ex, expc, s4)
+    ensures user_regs(s4.regs) == user_regs(s3.regs)
+    ensures OperandContents(s4, OLR) == expc
+{
+    lemma_evalExceptionTaken_Mode(s3, ex, expc, s4);
+}
+
+
+lemma lemma_preEntryUserRegs(
+    s1:state, s1':state, ret1:SvcReturnRegs, rd1:PageDb,
+    s2:state, s2':state, ret2:SvcReturnRegs, rd2:PageDb,
+    disp:PageNr
+)
+    requires ValidState(s1) && ValidState(s1')
+    requires ValidState(s2) && ValidState(s2')
+    requires user_regs(s1.regs) == user_regs(s2.regs)
+    requires ret1 == ret2 
+    requires preEntryReturn(s1, s1', ret1, rd1, disp)
+    requires preEntryReturn(s2, s2', ret2, rd2, disp)
+    ensures  user_regs(s1'.regs) == user_regs(s2'.regs)
+{
+    assert s1'.regs[R0] == s2'.regs[R0];
+    assert s1'.regs[R1] == s2'.regs[R1];
+    assert s1'.regs[R2] == s2'.regs[R2];
+    assert s1'.regs[R3] == s2'.regs[R3];
+    assert s1'.regs[R4] == s2'.regs[R4];
+    assert s1'.regs[R5] == s2'.regs[R5];
+    assert s1'.regs[R6] == s2'.regs[R6];
+    assert s1'.regs[R7] == s2'.regs[R7];
+    assert s1'.regs[R8] == s2'.regs[R8];
+    forall( r | r in {R9, R10, R11, R12, LR(User), SP(User)} )
+        ensures s1.regs[r] == s2.regs[r]
+    {
+        assert r in USER_REGS();
+        assert user_regs(s1.regs) == user_regs(s2.regs);
+        assert user_regs(s1.regs)[r] == user_regs(s2.regs)[r];
+    }
+    assert s1'.regs[R9] == s2'.regs[R9];
+    assert s1'.regs[R10] == s2'.regs[R10];
+    assert s1'.regs[R11] == s2'.regs[R11];
+    assert s1'.regs[R12] == s2'.regs[R12];
+    assert s1'.regs[LR(User)] == s2'.regs[LR(User)];
+    assert s1'.regs[SP(User)] == s2'.regs[SP(User)];
+}
+
+predicate spsr_same(s1:state, s2:state)
+    requires ValidState(s1) && ValidState(s2)
+    requires mode_of_state(s1) != User
+    requires mode_of_state(s2) != User
+{
+    reveal ValidSRegState();
+    var spsr1 := spsr(mode_of_state(s1));
+    var spsr2 := spsr(mode_of_state(s2));
+    s1.sregs[spsr1] == s2.sregs[spsr2]
+}
+
+predicate cpsr_same(s1:state, s2:state)
+    requires ValidState(s1) && ValidState(s2)
+{
+    reveal ValidSRegState();
+    s1.sregs[cpsr] == s2.sregs[cpsr] &&
+    s1.conf.cpsr == s2.conf.cpsr
+}
+
+lemma lemma_eval_cpsrs(
+s11: state, s1':state, s12: state, 
+s21: state, s2':state, s22: state)
+    requires ValidState(s11) && ValidState(s12) && ValidState(s1')
+    requires ValidState(s21) && ValidState(s22) && ValidState(s2')
+    requires equivStates(s11, s1') && evalEnterUserspace(s1', s12)
+    requires equivStates(s21, s2') && evalEnterUserspace(s2', s22)
+    requires mode_of_state(s11) != User && mode_of_state(s21) != User
+    requires spsr_same(s11, s21)
+    ensures  cpsr_same(s12, s22)
+{
+    assert equivStates(s11, s1') && evalEnterUserspace(s1', s12);
+    assert equivStates(s21, s2') && evalEnterUserspace(s2', s22);
+    var (m1, m2) := (mode_of_state(s1'), mode_of_state(s2'));
+    var (spsr1, spsr2) := (OSReg(spsr(m1)), OSReg(spsr(m2)));
+    assert OperandContents(s1', spsr1) == OperandContents(s2', spsr2);
+    var (spsr1v, spsr2v) :=
+        (OperandContents(s1', spsr1), OperandContents(s2', spsr2));
+    assert evalUpdate(takestep(s1'), OSReg(cpsr), spsr1v, s12);
+    assert evalUpdate(takestep(s2'), OSReg(cpsr), spsr2v, s22);
+}
+
+lemma lemma_svcHandled_loweq_pdb(
+    s1: state, d1: PageDb, d1': PageDb,
+    s2: state, d2: PageDb, d2': PageDb, dispPg: PageNr, atkr: PageNr)
+    requires 
+        validPageDb(d1) &&
+        validPageDb(d2) &&
+        validPageDb(d1') &&
+        validPageDb(d2') &&
+        validDispatcherPage(d1, dispPg) &&
+        validDispatcherPage(d2, dispPg)
+    requires ValidState(s1) && mode_of_state(s1) != User
+    requires ValidState(s2) && mode_of_state(s2) != User
+    requires isReturningSvc(s1) && isReturningSvc(s2)
+    requires finalDispatcher(d1, dispPg) && finalDispatcher(d2, dispPg)
+    requires d1' == svcHandled(s1, d1, dispPg).1 
+    requires d2' == svcHandled(s2, d2, dispPg).1
+    requires user_regs(s1.regs) == user_regs(s2.regs)
+    requires atkr_entry(d1, d2, dispPg, atkr)
+    requires loweq_pdb(d1, d2, atkr)
+    ensures  atkr_entry(d1', d2', dispPg, atkr)
+    ensures  loweq_pdb(d1', d2', atkr)
+    ensures  svcHandled(s1, d1, dispPg).0 == svcHandled(s2, d2, dispPg).0
+{
+
+    var call := OperandContents(s1, OReg(R0));
+    var user_words1 := [s1.regs[R1], s1.regs[R2], s1.regs[R3], s1.regs[R4],
+        s1.regs[R5], s1.regs[R6], s1.regs[R7], s1.regs[R8]];
+    var user_words2 := [s2.regs[R1], s2.regs[R2], s2.regs[R3], s2.regs[R4],
+        s2.regs[R5], s2.regs[R6], s2.regs[R7], s2.regs[R8]];
+
+    assert user_words1 == user_words2 by {
+        assert R1 in USER_REGS();
+        assert R2 in USER_REGS();
+        assert R3 in USER_REGS();
+        assert R4 in USER_REGS();
+        assert R5 in USER_REGS();
+        assert R6 in USER_REGS();
+        assert R7 in USER_REGS();
+        assert R8 in USER_REGS();
+        assert R1 in user_regs(s1.regs);
+        assert R1 in user_regs(s2.regs);
+        assert R2 in user_regs(s1.regs);
+        assert R2 in user_regs(s2.regs);
+        assert R3 in user_regs(s1.regs);
+        assert R3 in user_regs(s2.regs);
+        assert R4 in user_regs(s1.regs);
+        assert R4 in user_regs(s2.regs);
+        assert R5 in user_regs(s1.regs);
+        assert R5 in user_regs(s2.regs);
+        assert R6 in user_regs(s1.regs);
+        assert R6 in user_regs(s2.regs);
+        assert R7 in user_regs(s1.regs);
+        assert R7 in user_regs(s2.regs);
+        assert R8 in user_regs(s1.regs);
+        assert R8 in user_regs(s2.regs);
+        // There's no good ascii version of upside-down face emoji,
+        // but if there was, it would go here.
+    }
+    var retRegs1 := svcHandled(s1, d1, dispPg).0;
+    var retRegs2 := svcHandled(s2, d2, dispPg).0;
+    lemma_svcHandled_validPageDb(s1, d1, dispPg, retRegs1, d1');
+    lemma_svcHandled_validPageDb(s2, d2, dispPg, retRegs2, d2');
+
+    assert OperandContents(s1, OReg(R0)) ==
+        OperandContents(s2, OReg(R0)) by {
+           assert R0 in USER_REGS(); 
+           assert R0 in user_regs(s1.regs);
+           assert R0 in user_regs(s2.regs);
+        }
+    if( call  == KOM_SVC_ATTEST ) {
+        assert d1' == d1;
+        assert d2' == d2;
+        reveal loweq_pdb();
+    } else if( call == KOM_SVC_VERIFY_STEP0 || call  == KOM_SVC_VERIFY_STEP1 ) {
+        assert d1[dispPg].entry == d2[dispPg].entry &&
+            d1'[dispPg].entry == d2'[dispPg].entry &&
+            d1'[dispPg].addrspace == d2'[dispPg].addrspace by {
+            reveal loweq_pdb();
+        }
+        forall (n: PageNr | n != dispPg )
+            ensures d1'[n] == d1[n]
+            ensures d2'[n] == d2[n] 
+            ensures pgInAddrSpc(d1, n, atkr) ==> 
+                pgInAddrSpc(d1', n, atkr)
+            ensures pgInAddrSpc(d2, n, atkr) ==> 
+                pgInAddrSpc(d2', n, atkr)
+            {
+                assert loweq_pdb(d1, d2, atkr);
+                if(d1[n].PageDbEntryTyped? && d1[n].addrspace == atkr){
+                    assert d1'[n].PageDbEntryTyped? &&
+                        d1'[n].addrspace == atkr;
+                }
+                reveal loweq_pdb();
+            }
+
+        reveal loweq_pdb();
+        assert loweq_pdb(d1', d2', atkr);
+        assert user_words1 == user_words2;
+    } else if( call == KOM_SVC_VERIFY_STEP2) {
+        var dummy:word := 0;
+        var hmac1 := svcHmacVerify(s1, d1, dispPg);
+        var hmac2 := svcHmacVerify(s2, d2, dispPg);
+        assert hmac1 == hmac2 by { reveal loweq_pdb(); }
+        var ok := if user_words1 == hmac1 then 1 else 0;
+        assert retRegs1 == (KOM_ERR_SUCCESS, ok, dummy, dummy, dummy, dummy, 
+            dummy, dummy, dummy);
+        assert retRegs2 == (KOM_ERR_SUCCESS, ok, dummy, dummy, dummy, dummy, 
+            dummy, dummy, dummy);
+        assert retRegs1 == retRegs2;
+        assert d1' == d1;
+        assert d2' == d2;
+        reveal loweq_pdb();
+    } else if (call == KOM_SVC_MAP_DATA) {
+        reveal loweq_pdb();
+    } else if (call == KOM_SVC_UNMAP_DATA) {
+        reveal loweq_pdb();
+    } else if (call == KOM_SVC_INIT_L2PTABLE) {
+        reveal loweq_pdb();
+    } else {
+        assert d1' == d1;
+        assert d2' == d2;
+        reveal loweq_pdb();
+    }
+}
+
+lemma {:timeLimitMultiplier 4}
+lemma_validEnclaveStepPrime_conf(
+s11: state, d11: PageDb, s14:state, d14:PageDb, r1:state, rd1:PageDb,
+s21: state, d21: PageDb, s24:state, d24:PageDb, r2:state, rd2:PageDb,
+dispPg:PageNr, retToEnclave1:bool, retToEnclave2:bool, atkr: PageNr
+)
+    requires ValidState(s11) && ValidState(s21) &&
+             ValidState(r1)  && ValidState(r2)  &&
+             validPageDb(d11) &&
+             validPageDb(d21) && 
+             validPageDb(d14) && 
+             validPageDb(d24) && 
+             validPageDb(rd1) && 
+             validPageDb(rd2) && 
+             SaneConstants()
+    requires atkr_entry(d11, d21, dispPg, atkr)
+    requires validEnclaveExecutionStep'(s11,d11,s14,d14,r1,rd1,dispPg,retToEnclave1)
+    requires validEnclaveExecutionStep'(s21,d21,s24,d24,r2,rd2,dispPg,retToEnclave2)
+    requires OperandContents(s11, OLR) == OperandContents(s21, OLR)
+    requires user_regs(s11.regs) == user_regs(s21.regs)
+    requires InsecureMemInvariant(s11, s21)
+    requires loweq_pdb(d11, d21, atkr)
+    requires s11.conf.nondet == s21.conf.nondet
+    requires mode_of_state(s11) != User && mode_of_state(s21) != User
+    requires spsr_same(s11, s21)
+    requires s11.conf.scr == s21.conf.scr;
+    ensures  atkr_entry(rd1, rd2, dispPg, atkr)
+    ensures  loweq_pdb(rd1, rd2, atkr)
+    ensures  InsecureMemInvariant(r1, r2)
+    ensures  retToEnclave1 == retToEnclave2
+    ensures  !retToEnclave1 ==> same_ret(r1, r2)
+    ensures  retToEnclave1 ==> r1.conf.scr == r2.conf.scr
+    ensures  retToEnclave1 ==> r1.conf.nondet == r2.conf.nondet
+    ensures  retToEnclave1 ==> OperandContents(r1, OLR) == OperandContents(r2, OLR)
+    ensures  retToEnclave1 ==> user_regs(r1.regs) == user_regs(r2.regs)
+{                        
+
+    assert l1pOfDispatcher(d11, dispPg) == l1pOfDispatcher(d21, dispPg) by
+        { reveal loweq_pdb(); }
+    var l1p := l1pOfDispatcher(d11, dispPg);
+
+    assert dataPagesCorrespond(s11.m, d11);
+    assert dataPagesCorrespond(s21.m, d21);
+    
+    assert userspaceExecutionAndException(s11, s14);
+    assert userspaceExecutionAndException(s21, s24);
+
+    reveal userspaceExecutionAndException();
+
+    var s1', s12 :| userspaceExecutionAndException'(s11, s1', s12, s14);
+    var s2', s22 :| userspaceExecutionAndException'(s21, s2', s22, s24);
+
+    var pc1 := OperandContents(s11, OLR);
+    var pc2 := OperandContents(s21, OLR);
+    
+    var (s13, expc1, ex1) := userspaceExecutionFn(s12, pc1);
+    var (s23, expc2, ex2) := userspaceExecutionFn(s22, pc2);
+
+    assert s13.conf.nondet == s23.conf.nondet by
+    {
+        reveal userspaceExecutionFn();
+        assert s13.conf.nondet == nondet_int(s12.conf.nondet, NONDET_GENERATOR());
+        assert s23.conf.nondet == nondet_int(s22.conf.nondet, NONDET_GENERATOR());
+    }
+
+    assert s12.m == s11.m;
+    assert s22.m == s21.m;
+    assert cpsr_same(s12, s22) by {
+        lemma_eval_cpsrs(s11, s1', s12, s21, s2', s22);
+    }
+
+    assert pageTableCorresponds(s12, d11, l1p) &&
+        pageTableCorresponds(s22, d21, l1p) by
+    { 
+        assert pageTableCorresponds(s11, d11, l1p);
+        assert pageTableCorresponds(s21, d21, l1p);
+        reveal pageTableCorresponds();
+    }
+
+    var pt1 := ExtractAbsPageTable(s12);
+    var pt2 := ExtractAbsPageTable(s22);
+    lemma_userStatesEquiv_atkr(
+        s11, s1', s12, s14, pc1, pt1, d11,
+        s21, s2', s22, s24, pc2, pt2, d21,
+        dispPg, atkr, l1p);
+
+    var user_state1 := user_visible_state(s12, pc1, pt1.v);
+    var user_state2 := user_visible_state(s22, pc2, pt2.v);
+
+    assert ex1 == ex2 by {
+        reveal userspaceExecutionFn();
+
+        assert s12.conf.cpsr.f == s22.conf.cpsr.f;
+        assert s12.conf.cpsr.i == s22.conf.cpsr.i;
+        
+        assert ex1 == nondet_exception(s12.conf.nondet, user_state1, s12.conf.cpsr.f, s12.conf.cpsr.i);
+        assert ex2 == nondet_exception(s22.conf.nondet, user_state2, s22.conf.cpsr.f, s22.conf.cpsr.i);
+    }
+
+    assert user_regs(s13.regs) == user_regs(s23.regs) by {
+        var hr1 := havocUserRegs(s12.conf.nondet, user_state1, s12.regs);
+        var hr2 := havocUserRegs(s22.conf.nondet, user_state2, s22.regs);
+        assert s13.regs == hr1 by
+            { reveal userspaceExecutionFn(); }
+        assert s23.regs == hr2 by
+            { reveal userspaceExecutionFn(); }
+        assert user_state1 == user_state2;
+        assert s12.conf.nondet == s22.conf.nondet;
+        forall (r | r in USER_REGS() )
+            ensures hr1[r] ==
+                nondet_private_word(s12.conf.nondet, user_state1, NONDET_REG(r))
+            ensures hr2[r] ==
+                nondet_private_word(s22.conf.nondet, user_state2, NONDET_REG(r))
+            ensures hr1[r] == hr2[r]
+            ensures user_regs(hr1)[r] == user_regs(hr2)[r]
+        {
+        }
+        lemma_user_regs_domain(hr1, user_regs(hr1));
+        lemma_user_regs_domain(hr2, user_regs(hr2));
+        assert forall r :: r in user_regs(hr1) <==> r in user_regs(hr2);
+		assert forall r | r in user_regs(hr1) :: user_regs(hr1)[r] == user_regs(hr2)[r];
+
+		eqregs(user_regs(hr1), user_regs(hr2));
+        assert user_regs(hr1) == user_regs(hr2);
+    }
+
+    assert expc1 == expc2 by { reveal userspaceExecutionFn(); }
+
+    assert s14.conf.ex == ex1 && s24.conf.ex == ex2;
+
+    assert s14.conf.nondet == s24.conf.nondet;
+
+    lemma_userspaceExec_atkr(
+        s11, s1', s12, s13, s14, d11, d14,
+        s21, s2', s22, s23, s24, d21, d24,
+        dispPg, atkr, l1p);
+
+    assert user_regs(s14.regs) == user_regs(s13.regs)
+        && user_regs(s24.regs) == user_regs(s23.regs) by
+    {
+        lemma_exceptionTakenRegs(s13, ex1, expc1, s14);
+        lemma_exceptionTakenRegs(s23, ex2, expc2, s24);
+    }
+
+    assert OperandContents(s14, OLR) == OperandContents(s24, OLR) by
+    {
+        lemma_exceptionTakenRegs(s13, ex1, expc1, s14);
+        lemma_exceptionTakenRegs(s23, ex2, expc2, s24);
+        assert expc1 == expc2;
+    }
+
+    assert retToEnclave1 == retToEnclave2 by {
+        assert retToEnclave1 == isReturningSvc(s14);
+        assert retToEnclave2 == isReturningSvc(s24);
+        reveal ValidRegState();
+        assert s14.conf.ex == s24.conf.ex;
+        assert R0 in USER_REGS();
+        assert R0 in user_regs(s14.regs) && R0 in user_regs(s24.regs);
+        assert user_regs(s14.regs) == user_regs(s24.regs);
+        assert s14.regs[R0] == s24.regs[R0];
+
+    }
+
+    assert s13.conf.scr == s12.conf.scr &&
+        s23.conf.scr == s22.conf.scr by
+    {
+        reveal userspaceExecutionFn();
+    }
+
+    assert s14.conf.scr == s24.conf.scr;
+
+    var retToEnclave := retToEnclave1;
+
+    assert InsecureMemInvariant(s13, s23) by {
+
+        var pt1 := ExtractAbsPageTable(s12);
+        var pt2 := ExtractAbsPageTable(s22);
+
+        assert pt1 == pt2 by {
+            lemma_eqpdb_pt_coresp(d11, d21, s12, s22, l1p, atkr);
+        }
+
+        lemma_insecure_mem_userspace(
+            s12, pc1, s13, expc1, ex1,
+            s22, pc2, s23, expc2, ex2);
+    }
+
+    assert validDispatcherPage(d14, dispPg) && validDispatcherPage(d24, dispPg);
+
+    if(retToEnclave) {
+        var retRegs1 := svcHandled(s14, d14, dispPg).0;
+        var retRegs2 := svcHandled(s24, d24, dispPg).0;
+
+        lemma_svcHandled_validPageDb(s14, d14, dispPg, retRegs1, rd1);
+        lemma_svcHandled_validPageDb(s24, d24, dispPg, retRegs2, rd2);
+
+        lemma_svcHandled_loweq_pdb(s14, d14, rd1,
+            s24, d24, rd2, dispPg, atkr);
+
+        assert r1.conf.nondet == r2.conf.nondet by {
+            assert s14.conf.nondet == s24.conf.nondet; 
+        }
+        assert loweq_pdb(rd1, rd2, atkr);
+        assert r1.conf.nondet == r2.conf.nondet;
+        assert retRegs1 == retRegs2;
+        assert user_regs(r1.regs) == user_regs(r2.regs) by
+        { 
+            lemma_preEntryUserRegs(
+                s14, r1, retRegs1, rd1,
+                s24, r2, retRegs2, rd2, dispPg
+            );
+        }
+        assert OperandContents(r1, OLR) == OperandContents(r2, OLR);
+    } else { // XXX same_ret
+        assert cpsr in s13.sregs && cpsr in s23.sregs &&
+            s13.sregs[cpsr] == s23.sregs[cpsr] by
+            { 
+                assert user_state1 == user_state2;
+                assert s12.conf.cpsr == s22.conf.cpsr;
+                var newpsr := nondet_psr(s12.conf.nondet, user_state1, s12.conf.cpsr);
+                reveal userspaceExecutionFn();
+                assert s13.sregs[cpsr] == newpsr;
+                assert s23.sregs[cpsr] == newpsr;
+            }
+        assert mode_of_exception(s13.conf, ex1) ==
+            mode_of_exception(s23.conf, ex2) by
+            { 
+                assert s13.conf.scr.irq == s23.conf.scr.irq;
+                assert s13.conf.scr.fiq == s23.conf.scr.fiq;
+                reveal userspaceExecutionFn();
+            }
+
+        assert s14 == exceptionTakenFn(s13, ex1, expc1) by {
+            assert evalExceptionTaken(s13, ex1, expc1, s14);
+        }
+        assert s24 == exceptionTakenFn(s23, ex2, expc2) by {
+            assert evalExceptionTaken(s13, ex1, expc1, s14);
+        }
+        lemma_exceptionTaken_atkr(
+            s13, s14, ex1, expc1, 
+            s23, s24, ex2, expc2);
+        lemma_exceptionHandled_atkr(s14, d14, rd1, s24, d24, rd2,
+             r1.regs[R0], r1.regs[R1], r2.regs[R0], r2.regs[R1],
+             dispPg, atkr); // XXX validDispPg(dispPg)
+
+        assert loweq_pdb(rd1, rd2, atkr);
+    }
+}
+
+lemma lemma_exceptionTaken_atkr(
+    s13: state, s14: state, ex1:exception, pc1:word,
+    s23: state, s24: state, ex2:exception, pc2:word
+)
+    requires ValidState(s13) && ValidState(s23) &&
+        ValidState(s14) && ValidState(s24);
+    requires user_regs(s13.regs) == user_regs(s23.regs)
+    requires ex1 == ex2 && pc1 == pc2
+    requires cpsr in s13.sregs && cpsr in s23.sregs &&
+        s13.sregs[cpsr] == s23.sregs[cpsr]
+    requires mode_of_exception(s13.conf, ex1) ==
+        mode_of_exception(s23.conf, ex2)
+    requires ValidPsrWord(psr_of_exception(s13, ex1))
+    requires ValidPsrWord(psr_of_exception(s23, ex2))
+    requires s14 == exceptionTakenFn(s13, ex1, pc1)
+    requires s24 == exceptionTakenFn(s23, ex2, pc2)
+    ensures user_regs(s14.regs) == user_regs(s24.regs)
+    ensures mode_of_state(s14) != User && mode_of_state(s24) != User
+    ensures mode_of_state(s14) == mode_of_state(s24)
+    ensures lr_spsr_same(s14, s24);
+{
+    assert user_regs(s14.regs) == user_regs(s24.regs) by {
+        var newmode := mode_of_exception(s13.conf, ex1);
+        assert s14.regs == s13.regs[LR(newmode) := pc1];
+        assert s24.regs == s23.regs[LR(newmode) := pc1];
+        assert forall r :: r in user_regs(s14.regs) <==> r in user_regs(s24.regs);
+        assert forall r :: r in user_regs(s14.regs) <==> r in user_regs(s13.regs);
+        forall( r | r in user_regs(s14.regs)) 
+            ensures user_regs(s24.regs) == user_regs(s14.regs)
+        {
+            assert user_regs(s13.regs) == user_regs(s23.regs);
+            if(r != LR(newmode)) {
+                assert s14.regs[r] == s13.regs[r];
+                assert s24.regs[r] == s23.regs[r];
+                assert s13.regs[r] == s23.regs[r];
+            } else {
+            }
+        }
+        eqregs(user_regs(s24.regs), user_regs(s14.regs));
+    }
+    lemma_evalExceptionTaken_Mode(s13, ex1, pc1, s14);
+}
+
+// This is just for the reveal
+predicate lr_spsr_same(s1:state, s2:state)
+    requires ValidState(s1) && ValidState(s2)
+    requires mode_of_state(s1) != User && mode_of_state(s2) != User
+{
+    reveal ValidRegState();
+    reveal ValidSRegState();
+    s1.regs[LR(mode_of_state(s1))] == s2.regs[LR(mode_of_state(s2))] &&
+    s1.sregs[spsr(mode_of_state(s1))] == s2.sregs[spsr(mode_of_state(s2))]
+}
+
+lemma lemma_exceptionHandled_atkr(
+s1: state, d1: PageDb, d1': PageDb, s2: state, d2: PageDb, d2': PageDb,
+dispPg: PageNr, atkr: PageNr, 
+r01: word, r11: word, r02: word, r12: word)
+    requires ValidState(s1) && ValidState(s2) &&
+             validPageDb(d1') && validPageDb(d2') &&
+             validPageDb(d1) && validPageDb(d2) && SaneConstants()
+    requires s1.conf.nondet == s2.conf.nondet;
+    requires mode_of_state(s1) != User && mode_of_state(s2) != User
+    requires mode_of_state(s1) == mode_of_state(s2)
+    requires lr_spsr_same(s1, s2)
+    requires validDispatcherPage(d1, dispPg) && validDispatcherPage(d2, dispPg) 
+    requires (r01, r11, d1') == exceptionHandled(s1, d1, dispPg)
+    requires (r02, r12, d2') == exceptionHandled(s2, d2, dispPg)
+    requires atkr_entry(d1, d2, dispPg, atkr)
+    requires loweq_pdb(d1, d2, atkr)
+    requires user_regs(s1.regs) == user_regs(s2.regs)
+    requires s1.conf.ex == s2.conf.ex
+    ensures  loweq_pdb(d1', d2', atkr)
+    ensures  atkr_entry(d1', d2', dispPg, atkr)
+    ensures  r01 == r02 && r11 == r12
+{
+    reveal loweq_pdb();
+    var ex := s1.conf.ex;
+    forall (n : PageNr |  n != dispPg)
+        ensures d1'[n] == d1[n];
+        ensures d2'[n] == d2[n];
+        ensures pgInAddrSpc(d1, n, atkr) <==>
+            pgInAddrSpc(d1', n, atkr)
+        ensures pgInAddrSpc(d2, n, atkr) <==>
+            pgInAddrSpc(d2', n, atkr)
+    {
+    }
+
+    assert forall n : PageNr :: pgInAddrSpc(d1, n, atkr) <==>
+        pgInAddrSpc(d2, n, atkr);
+
+    forall( n : PageNr | n != dispPg &&
+        pgInAddrSpc(d1, n, atkr) )
+    ensures d1'[n] == d2'[n]
+    {
+    }
+
+    if( ex.ExSVC? ) {
+        assert d1'[dispPg].entry == d2'[dispPg].entry;
+        assert r01 == r02;
+        assert R1 in USER_REGS();
+        assert user_regs(s1.regs)[R1] == user_regs(s2.regs)[R1];
+        assert s1.regs[R1] == s2.regs[R1];
+        assert r11 == r12;
+    } else if( ex.ExAbt? || ex.ExUnd? ) {
+        assert d1'[dispPg].entry == d2'[dispPg].entry;
+        assert r01 == r02;
+        assert r11 == r12;
+    } else {
+        var pc1 := TruncateWord(OperandContents(s1, OLR) - 4);
+        var pc2 := TruncateWord(OperandContents(s2, OLR) - 4);
+        assert pc1 == pc2;
+        reveal ValidSRegState();
+        var psr1 := s1.sregs[spsr(mode_of_state(s1))];
+        var psr2 := s2.sregs[spsr(mode_of_state(s2))];
+        assert psr1 == psr2;
+        var ctxt1' := DispatcherContext(user_regs(s1.regs), pc1, psr1);
+        var ctxt2' := DispatcherContext(user_regs(s2.regs), pc2, psr2);
+        assert user_regs(s1.regs) == user_regs(s2.regs);
+        assert ctxt1' == ctxt2';
+        assert d1'[dispPg].entry == d2'[dispPg].entry;
+    }
+}
+
+lemma
+    {:fuel userspaceExecutionAndException', 0}
+    {:fuel ExtractAbsPageTable, 0}
+    {:fuel l1pOfDispatcher, 0}
+lemma_userMemEquiv_atkr(
+s11: state, s1':state, s12: state, s14: state,
+pc1: word, pt1: Maybe<AbsPTable>, d1: PageDb,
+s21: state, s2':state, s22: state, s24: state,
+pc2: word, pt2: Maybe<AbsPTable>, d2: PageDb,
+dispPg: PageNr, atkr: PageNr, l1p: PageNr)
+    requires ValidState(s11) && ValidState(s12) && ValidState(s14)
+    requires ValidState(s21) && ValidState(s22) && ValidState(s24)
+    requires validPageDb(d1) && validPageDb(d2)
+    requires SaneConstants()
+    requires valAddrPage(d1, atkr) && valAddrPage(d2, atkr)
+    requires loweq_pdb(d1, d2, atkr)
+    requires s12.conf.nondet == s22.conf.nondet
+    requires userspaceExecutionAndException'(s11, s1', s12, s14)
+    requires userspaceExecutionAndException'(s21, s2', s22, s24)
+    requires pc1 == OperandContents(s11, OLR) && pc2 == OperandContents(s21, OLR);
+    requires pt1 == ExtractAbsPageTable(s12) && pt2 == ExtractAbsPageTable(s22);
+    requires nonStoppedL1(d1, l1p) && nonStoppedL1(d2, l1p)
+    requires atkr_entry(d1, d2, dispPg, atkr)
+    requires l1pOfDispatcher(d1, dispPg) == l1pOfDispatcher(d2, dispPg) == l1p
+    requires !stoppedAddrspace(d1[atkr]) && !stoppedAddrspace(d2[atkr])
+    requires user_regs(s11.regs) == user_regs(s21.regs);
+    requires pc1 == pc2;
+    requires 
+        pageTableCorresponds(s12, d1, l1p) &&
+        pageTableCorresponds(s22, d2, l1p) &&
+        dataPagesCorrespond(s12.m, d1) &&
+        dataPagesCorrespond(s22.m, d2)
+    requires valAddrPage(d1, atkr) && valAddrPage(d2, atkr)
+        && d1[atkr].entry.l1ptnr == d2[atkr].entry.l1ptnr == l1p
+    requires pgInAddrSpc(d1, l1p, atkr) && pgInAddrSpc(d2, l1p, atkr)
+    ensures pt1.Just? && pt2.Just?
+    ensures user_mem(pt1.v, s12.m) == user_mem(pt2.v, s22.m)
+{
+    assert pt1.Just? && pt2.Just?
+        && ExtractAbsPageTable(s11).Just?
+        && ExtractAbsPageTable(s21).Just? by
+    {
+        assert{:fuel ExtractAbsPageTable, 1}{:fuel userspaceExecutionAndException', 1}
+            pt1.Just? && pt2.Just?;
+        assert{:fuel userspaceExecutionAndException', 1}
+            ExtractAbsPageTable(s11).Just? && ExtractAbsPageTable(s21).Just? by 
+            {
+                assert evalUserExecution(s1', s12, s14) &&
+                    evalUserExecution(s2', s22, s24);
+                assert ExtractAbsPageTable(s12).Just? &&
+                    ExtractAbsPageTable(s22).Just?;
+                assert {:fuel ExtractAbsPageTable, 1}
+                    ExtractAbsPageTable(s1').Just? && 
+                        ExtractAbsPageTable(s2').Just?;
+                assert {:fuel ExtractAbsPageTable, 1}
+                    ExtractAbsPageTable(s11).Just? &&
+                        ExtractAbsPageTable(s21).Just?;
+            }
+    }
+
+    lemma_eqpdb_pt_coresp(d1, d2, s12, s22, l1p, atkr);
+
+    forall a:addr | ValidMem(a) && a in TheValidAddresses() && addrIsSecure(a)
+            && PageBase(a) in AllPagesInTable(pt1.v)
+        ensures a in s12.m.addresses
+        ensures a in s22.m.addresses
+        ensures s12.m.addresses[a] == s22.m.addresses[a]
+    {
+        lemma_data_eqpdb_to_addrs(d1, d2, s12, s22, a, atkr, l1p);
+    }
+}
+
+lemma lemma_userStatesEquiv_atkr(
+s11: state, s1':state, s12: state, s14: state,
+pc1: word, pt1: Maybe<AbsPTable>, d1: PageDb,
+s21: state, s2':state, s22: state, s24: state,
+pc2: word, pt2: Maybe<AbsPTable>, d2: PageDb,
+dispPg: PageNr, atkr: PageNr, l1p: PageNr)
+    requires ValidState(s11) && ValidState(s12) && ValidState(s14)
+    requires ValidState(s21) && ValidState(s22) && ValidState(s24)
+    requires validPageDb(d1) && validPageDb(d2)
+    requires SaneConstants()
+    requires valAddrPage(d1, atkr) && valAddrPage(d2, atkr)
+    requires loweq_pdb(d1, d2, atkr)
+    requires s12.conf.nondet == s22.conf.nondet
+    requires userspaceExecutionAndException'(s11, s1', s12, s14)
+    requires userspaceExecutionAndException'(s21, s2', s22, s24)
+    requires pc1 == OperandContents(s11, OLR) && pc2 == OperandContents(s21, OLR);
+    requires pt1 == ExtractAbsPageTable(s12) && pt2 == ExtractAbsPageTable(s22);
+    requires nonStoppedL1(d1, l1p) && nonStoppedL1(d2, l1p)
+    requires atkr_entry(d1, d2, dispPg, atkr)
+    requires l1pOfDispatcher(d1, dispPg) == l1pOfDispatcher(d2, dispPg) == l1p
+    requires !stoppedAddrspace(d1[atkr]) && !stoppedAddrspace(d2[atkr])
+    requires user_regs(s11.regs) == user_regs(s21.regs);
+    requires pc1 == pc2;
+    requires 
+        pageTableCorresponds(s12, d1, l1p) &&
+        pageTableCorresponds(s22, d2, l1p) &&
+        dataPagesCorrespond(s12.m, d1) &&
+        dataPagesCorrespond(s22.m, d2)
+    requires valAddrPage(d1, atkr) && valAddrPage(d2, atkr)
+        && d1[atkr].entry.l1ptnr == d2[atkr].entry.l1ptnr == l1p
+    requires pgInAddrSpc(d1, l1p, atkr) && pgInAddrSpc(d2, l1p, atkr)
+    ensures pt1.Just? && pt2.Just?
+    ensures  user_visible_state(s12, pc1, pt1.v) == user_visible_state(s22, pc2, pt2.v)
+{
+    lemma_userMemEquiv_atkr(
+        s11, s1', s12, s14, pc1, pt1, d1,
+        s21, s2', s22, s24, pc2, pt2, d2,
+        dispPg, atkr, l1p);
+}
+
+
+// TODO: move this to ptables.i.dfy, next to lemma_WritablePages
+lemma lemma_AllPages(d:PageDb, l1p:PageNr, pagebase:addr, pt:PageNr)
+    requires PhysBase() == KOM_DIRECTMAP_VBASE
+    requires validPageDb(d)
+    requires nonStoppedL1(d, l1p)
+    requires PageAligned(pagebase) && address_is_secure(pagebase)
+    requires pt == monvaddr_page(pagebase)
+    requires pagebase in AllPagesInTable(mkAbsPTable(d, l1p))
+    ensures d[pt].PageDbEntryTyped?;
+    ensures d[pt].entry.DataPage?;
+    ensures d[pt].addrspace == d[l1p].addrspace;
+{
+    assert validL1PTable(d, d[l1p].addrspace, d[l1p].entry.l1pt) by { reveal validPageDb(); }
+    var abspt := mkAbsPTable(d, l1p);
+    var l1pt := d[l1p].entry.l1pt;
+    var i, j :| 0 <= i < ARM_L1PTES && 0 <= j < ARM_L2PTES
+        && abspt[i].Just? && abspt[i].v[j].Just?
+        && pagebase == abspt[i].v[j].v.phys + PhysBase();
+    var p := monvaddr_page(pagebase);
+    reveal mkAbsPTable();
+    assert p == (abspt[i].v[j].v.phys - SecurePhysBase()) / PAGESIZE;
+    var n := i / 4;
+    assert l1pt[n].Just?;
+    var l2p := l1pt[n].v;
+    assert d[l2p].PageDbEntryTyped? && d[l2p].entry.L2PTable?
+        && wellFormedPageDbEntry(d[l2p])
+        && validL2PTable(d, d[l2p].addrspace, d[l2p].entry.l2pt)
+        by { reveal validPageDb(); }
+    var l2pt := d[l2p].entry.l2pt;
+    var pte := l2pt[(i%4)*ARM_L2PTES + j];
+    assert validL2PTE(d, d[l2p].addrspace, pte);
+    assert mkAbsPTE(pte) == abspt[i].v[j];
+    assert pte.SecureMapping?;
+}
+
+lemma lemma_data_eqpdb_to_addrs( d1:PageDb, d2:PageDb, s1: state, s2: state,
+a:addr, atkr:PageNr, l1p: PageNr)
+    requires validPageDb(d1) && validPageDb(d2)
+    requires ValidState(s1) && ValidState(s2) && SaneConstants()
+    requires valAddrPage(d1, atkr) && valAddrPage(d2, atkr)
+    requires loweq_pdb(d1, d2, atkr)
+    requires dataPagesCorrespond(s1.m, d1) && dataPagesCorrespond(s2.m, d2)
+    requires ExtractAbsPageTable(s1).Just?
+    requires ExtractAbsPageTable(s2).Just?
+    requires ValidMem(a)
+    requires a in TheValidAddresses()
+    requires addrIsSecure(a)
+    requires PageBase(a) in AllPagesInTable(ExtractAbsPageTable(s1).v)
+    requires PageBase(a) in AllPagesInTable(ExtractAbsPageTable(s2).v)
+    requires nonStoppedL1(d1, l1p) && nonStoppedL1(d2, l1p)
+    requires pgInAddrSpc(d1, l1p, atkr) && pgInAddrSpc(d2, l1p, atkr)
+    requires pageTableCorresponds(s1, d1, l1p)
+    requires pageTableCorresponds(s2, d2, l1p)
+    ensures a in s1.m.addresses
+    ensures a in s2.m.addresses
+    ensures s1.m.addresses[a] == s2.m.addresses[a]
+{
+    var p := lemma_secure_addrInPage(a);
+
+    assert PageBase(a) in AllPagesInTable(mkAbsPTable(d1, l1p))
+        && PageBase(a) in AllPagesInTable(mkAbsPTable(d2, l1p)) by
+        { reveal pageTableCorresponds(); }
+
+    lemma_AllPages(d1, l1p, PageBase(a), monvaddr_page(PageBase(a)));
+    lemma_AllPages(d2, l1p, PageBase(a), monvaddr_page(PageBase(a)));
+
+    assert a in addrsInPage(p, page_monvaddr(p)) by
+    {
+        var a0 := page_monvaddr(p);
+        var a1 := a0 + PAGESIZE;
+        var i := (a - a0) / WORDSIZE;
+        assert addrRangeSeq(a0, a1)[i] == a0 + WordsToBytes(i);
+    }
+    lemma_data_page_eqdb_to_addrs(d1, d2, s1, s2, p, a, atkr);
+}
+
+lemma lemma_data_page_eqdb_to_addrs( d1:PageDb, d2:PageDb, s1: state, s2: state,
+n:PageNr, a:addr, atkr:PageNr)
+    requires validPageDb(d1) && validPageDb(d2)
+    requires ValidState(s1) && ValidState(s2) && SaneConstants()
+    requires d1[n].PageDbEntryTyped? && d1[n].entry.DataPage?
+    requires d2[n].PageDbEntryTyped? && d2[n].entry.DataPage?
+    requires valAddrPage(d1, atkr) && valAddrPage(d2, atkr)
+    requires d1[n].addrspace == atkr && d2[n].addrspace == atkr
+    requires loweq_pdb(d1, d2, atkr)
+    requires a in addrsInPage(n, page_monvaddr(n))
+    requires dataPagesCorrespond(s1.m, d1) && dataPagesCorrespond(s2.m, d2)
+    ensures s1.m.addresses[a] == s2.m.addresses[a]
+{
+    reveal loweq_pdb();
+    reveal pageDbDataCorresponds();
+
+    // trigger i in pageDbDataCorresponds:
+    var i := (a - page_monvaddr(n)) / WORDSIZE;
+    assert d1[n].entry.contents[i] == d2[n].entry.contents[i];
+}
+
+lemma lemma_eqpdb_pt_coresp(d1: PageDb, d2: PageDb, s1: state, s2: state,
+l1p:PageNr, atkr: PageNr)
+    requires validPageDb(d1) && validPageDb(d2)
+    requires ValidState(s1) && ValidState(s2)
+    requires ValidState(s1) && ValidState(s2) && SaneConstants()
+    requires valAddrPage(d1, atkr) && valAddrPage(d2, atkr)
+    requires !stoppedAddrspace(d1[atkr]) && !stoppedAddrspace(d2[atkr])
+    requires loweq_pdb(d1, d2, atkr)
+    requires nonStoppedL1(d1, l1p) && nonStoppedL1(d2, l1p)
+    requires pageTableCorresponds(s1, d1, l1p)
+    requires pageTableCorresponds(s2, d2, l1p)
+    requires valAddrPage(d1, atkr) && valAddrPage(d2, atkr)
+        && d1[atkr].entry.l1ptnr == d2[atkr].entry.l1ptnr == l1p
+    requires pgInAddrSpc(d1, l1p, atkr) && pgInAddrSpc(d2, l1p, atkr)
+    ensures  ExtractAbsPageTable(s1) == ExtractAbsPageTable(s2)
+{
+    reveal pageTableCorresponds();
+    assert mkAbsPTable(d1, l1p) == mkAbsPTable(d2, l1p) by {
+        reveal loweq_pdb();
+        reveal validPageDb();
+        reveal mkAbsPTable();
+    }
+}
+
+lemma lemma_eqpdb_pt_coresp_not_atkr(d1: PageDb, d2: PageDb, s1: state, s2: state,
+    l1p:PageNr, asp: PageNr, atkr: PageNr)
+    requires validPageDb(d1) && validPageDb(d2)
+    requires ValidState(s1) && ValidState(s2)
+    requires ValidState(s1) && ValidState(s2) && SaneConstants()
+    requires valAddrPage(d1, asp ) && valAddrPage(d2, asp)
+    requires valAddrPage(d1, atkr) && valAddrPage(d2, atkr)
+    requires atkr != asp
+    requires loweq_pdb(d1, d2, atkr)
+    requires nonStoppedL1(d1, l1p) && nonStoppedL1(d2, l1p)
+    requires pageTableCorresponds(s1, d1, l1p)
+    requires pageTableCorresponds(s2, d2, l1p)
+    requires d1[asp].entry.l1ptnr == d2[asp].entry.l1ptnr == l1p
+    ensures  ExtractAbsPageTable(s1) == ExtractAbsPageTable(s2)
+{
+    reveal pageTableCorresponds();
+    assert mkAbsPTable(d1, l1p) == mkAbsPTable(d2, l1p) by {
+        reveal loweq_pdb();
+        reveal validPageDb();
+        reveal mkAbsPTable();
+    }
+}
+
+//-----------------------------------------------------------------------------
+// Resume
+//-----------------------------------------------------------------------------
+lemma lemma_resume_conf_ni(s1: state, d1: PageDb, s1':state, d1': PageDb,
+                               s2: state, d2: PageDb, s2':state, d2': PageDb,
+                               dispPage: word,
+                               atkr: PageNr)
+    requires ni_reqs(s1, d1, s1', d1', s2, d2, s2', d2', atkr)
+    requires smc_resume(s1, d1, s1', d1', dispPage)
+    requires smc_resume(s2, d2, s2', d2', dispPage)
+    requires conf_loweq(s1, d1, s2, d2, atkr)
+    requires loweq_pdb(d1, d2, atkr)
+    requires s1.conf.nondet == s2.conf.nondet
+    ensures  loweq_pdb(d1', d2', atkr)
+    ensures  same_ret(s1', s2')
+    ensures  InsecureMemInvariant(s1', s2')
+{
+    reveal loweq_pdb();
+    var e1, e2 := smc_enter_err(d1, dispPage, true), smc_enter_err(d2, dispPage, true);
+    assert e1 == e2;
+
+    if(e1 == KOM_ERR_SUCCESS) {
+        var asp1, asp2 := d1[dispPage].addrspace, d2[dispPage].addrspace;
+        assert asp1 == asp2;
+        if(asp1 == atkr) {
+            lemma_enter_conf_atkr_enter(s1, d1, s1', d1',
+                                       s2, d2, s2', d2',
+                                       dispPage, 0, 0, 0, 
+                                       atkr, true);
+        } else {
+            lemma_enter_loweq_pdb_not_atkr(s1, d1, s1', d1',
+                                           s2, d2, s2', d2',
+                                           dispPage, 0, 0, 0,
+                                           asp1, atkr, true);
+        }
+    } 
+}
